%\documentclass[trans]{beamer}
\documentclass{beamer}

\usetheme{Singapore}
\setbeamercovered{transparent} 
\usepackage{amsmath}
\usepackage{stmaryrd}
\usepackage{src/prooftree}

\usepackage[all]{xy}

\def\igual{=}
\def\caixa#1{\medskip
  \begin{center}
  \fbox{\begin{minipage}{0.9\textwidth}\protect{#1}\end{minipage}}
  \end{center}}
  
\def\hdd{\fun{hd}}
\def\tll{\fun{tl}}
\def\swap{\fuc{swap}}
\def\twist{\fuc{twist}}
  %------ using color ---------------------------------------------------------
\usepackage{color}
%input{rgb}
\def\black{\color{black}}
\def\blue{\color{blue}}
\def\red{\color{red}}

\def\true{\fuc{true}}
\def\false{\fuc{false}}
%\def\dimp{\mathbin{\Leftrightarrow}}
\def\dimp{\mathbin{\equiv}}

\def\imp{\mathbin{\Rightarrow}}
\def\rimp{\mathbin{\Leftarrow}}
\def\limp{\mathbin{\multimap}}
\newcommand{\sse}{\mathbin{\, \operatorname{\textsf{iff}} \,}}
\def\e{\mathbin{\wedge}}
\def\ou{\mathbin{\vee}}

  
  \input{src/newmacros.mac}
  
  
\title{
	Mathematics for Computer Science
}
\author{ Jos\'{e} Proen\c{c}a \& Alexandre Madeira\\ (slides from Luis Soares Barbosa)\\ ~}

\institute{
 \includegraphics[height=1.5cm]{img/HASLab-logo} \hspace{1cm}
 \includegraphics[height=1.5cm]{img/um} \hspace{1cm} 
 % \includegraphics[height=1.5cm]{UNU-EGOV}
 }
%\institute{HASLab INESC TEC \& Universidade do Minho \& UNU-EGOV - United Nations University \\
%Braga, Portugal}
\date{
\begin{tabular}{c}
\\
	\textbf{Propositional Calculus} \\  September-October,  2017
\\
\end{tabular}
}

\begin{document}

\frame[plain]{\titlepage}

\section{The calculus}

\begin{slide}{Calculus}



\begin{block}{Boolean expressions can be defined by}
\begin{itemize}
\item how they are evaluated (models)
\item how they can be manipulated (proofs)
\end{itemize}
\end{block}

\caixa{A calculus is a method or process of reasoning by calculation with symbols. }
\end{slide} 

\begin{slide}{Equational reasoning}
\begin{description}
\item[Axioms] i.e. boolean expressions that define basic manipulative properties of boolean operators
\item[Inference rules]
~\\

\begin{center}
\begin{prooftree}
P=Q, Q=R
\justifies
P = R
\thickness=0.08em
\using
{\text{(transitivity)}}
\end{prooftree}
\end{center}
\vspace{5mm}
\begin{center}
\begin{prooftree}
P= Q 
\justifies
E[z := P] = E[z := Q] 
\thickness=0.08em
\using
{\text{(Leibniz)}}
\end{prooftree}
\end{center}
\vspace{5mm}

\begin{center}
\begin{prooftree}
P
\justifies
P[z := Q] 
\thickness=0.08em
\using
{\text{(substitution)}}
\end{prooftree}
\end{center}
\vspace{5mm}

where $P,Q, ...$ are arbitrary Boolean expressions, and $p,q,r,z,...$ are Boolean variables.
\end{description}

\end{slide} 



\begin{slide}{Equational reasoning}
\begin{block}{Equivalence}
\begin{align*}
\text{($\dimp$ associativity)} && & ((p \dimp q) \dimp r) ~~\dimp~~ (p \dimp (q \dimp r))\\
\text{($\dimp$ commutativity)} &&  & p \dimp q ~~\dimp~~ q \dimp p \\
\text{($\dimp$ identity)} &&  & \true ~~\dimp~~ q \dimp q
\end{align*}
\end{block}
\end{slide} 


\begin{slide}{Equational reasoning}
\begin{block}{Negation}
\begin{align*}
\text{($\false$ definition)} && & \false ~~\dimp~~ \neg \true\\
\text{($\neg$ distributivity over $\dimp$)} &&  & \neg(p \dimp q) ~~\dimp~~ \neg p \dimp q\\
\text{($\not\equiv$ definition)} &&  & (p \not\equiv q) ~~\dimp~~ \neg(p \dimp q)
\end{align*}
\end{block}

\begin{block}{\dkb{De Morgan laws} -- from the duality meta-theorem}
\begin{align*}
\text{($\e$ negation)} && \neg (p \e q) &\dimp (\neg p \ou \neg q)
\\
\text{($\ou$ negation)} && \neg (p \ou q) &\dimp (\neg p \e \neg q)
\end{align*}
\end{block}
\end{slide} 

\begin{slide}{Equational reasoning}
\begin{block}{Disjunction}
\begin{align*}
\text{($\ou$ commutativity)} && & p \ou q ~~\dimp~~ q \ou p\\
\text{($\ou$ associativity)} && &(p \ou q) \ou r ~~\dimp~~ p\ou (q \ou r)\\
\text{($\ou$ idempotency)} && & p \ou p ~~\dimp~~ p\\
\text{($\ou$ distributivity over $\dimp$)} &&  & p \ou (q \dimp r) ~~\dimp~~ (p\ou q) \dimp (p \ou r)  \\
\text{(excluded middle)} &&  & p \ou \neg p ~~\dimp~~ \true
\end{align*}
\end{block}


\end{slide} 

\begin{slide}{Equational reasoning}
\begin{block}{Conjunction}
\begin{align*}
\text{(golden rule)} && & p \e q ~~\dimp~~ p \dimp q \dimp p \ou q\\
\end{align*}
\end{block}
\end{slide}
% ("p false" means "q any")
% ("p true" means "q must be true")
%  --- p -> q

\begin{slide}{Equational reasoning}
\begin{block}{Implication}
\begin{align*}
\text{($\imp$ definition)} && & p \imp q ~~\dimp~~ p \ou q \dimp q\\
\text{(consequence)} && &p \rimp q ~~\dimp~~ q \imp p\\
\end{align*}
\end{block}
\end{slide} 

\section{Examples}
 \begin{slide}{Example}
\begin{center}
\fbox{Theorem: $\neg p \dimp q \dimp p \dimp \neg q$}
\end{center}
\begin{eqnarray*}
& & \neg p \dimp q \dimp p \dimp \neg q
%
\just \igual{ $\dimp$ associativity, commutativity }
%
(\neg p \dimp p) \dimp (q \dimp \neg q)
%
\just \igual{ $\neg$ distributivity over $\dimp$ }
%
\neg (p \dimp p) \dimp \neg (q \dimp q)
%
\just \igual{ $\dimp$ identity, $\false$ definition}
%
\false \dimp \false
%
\just \igual{ $\dimp$ identity}
%
\true
\end{eqnarray*}

\end{slide} 


\begin{slide}{Example}
\begin{center}
\fbox{Theorem: $p \ou  \true \dimp \true$}
\end{center}
\begin{eqnarray*}
& & p \ou  \true
%
\just \igual{ $\dimp$ identity }
%
p \ou  (p \dimp p)
%
\just \igual{ $\ou$ distributivity over $\dimp$ }
%
p \ou p \dimp p \ou p
%
\just \igual{ $\dimp$ identity}
%
\true
\end{eqnarray*}

\end{slide} 


\begin{slide}{Example}
\begin{center}
\fbox{Theorem: $p \ou q \dimp p \ou \neg q \dimp p$}
\end{center}
\begin{eqnarray*}
& & p \ou q \dimp p \ou \neg q \dimp p
%
\just \igual{ $\ou$ distributivity over $\dimp$ }
%
p \ou  (q \dimp \neg q) \dimp p
%
\just \igual{ $\neg$ distributivity over $\dimp$ }
%
p \ou \false \dimp p
%
\just \igual{ theorem - exercise below}
%
p \dimp p
%
\just \igual{ $\dimp$ identity }
%
\true
\end{eqnarray*}

\end{slide} 


\begin{slide}{Example}
\begin{center}
\fbox{Theorem: $p \e (\neg p \ou q) \dimp (p \e q)$}
\end{center}
\begin{eqnarray*}
& &p \e (\neg p \ou q)
%
\just \igual{ golden rule }
%
p \dimp \neg p \ou q \dimp p \ou \neg p \ou q
%
\just \igual{ $\dimp$ associativity, excluded middle }
%
p \dimp \neg p \ou q \dimp \true \ou q
%
\just \igual{ theorem above: $p \ou \true \dimp \true$}
%
p \dimp \neg p \ou q
%
\just \igual{ theorem above: $p \ou q \dimp p \ou \neg q \dimp p$}
%
p \dimp p \ou q \dimp q
%
\just \igual{ golden rule }
%
p \e q
\end{eqnarray*}

\end{slide} 


\begin{slide}{Example}
\begin{center}
\fbox{Theorem: $(p \e q) \e r \dimp p \e (q \e r) $}
\end{center}
\begin{eqnarray*}
& & (p \e q) \e r 
%
\just \igual{ golden rule }
%
(p \dimp q \dimp p \ou q) \e r
%
\just \igual{ golden rule }
%
(p \dimp q \dimp p \ou q) \dimp r \dimp ((p \dimp q \dimp p \ou q) \ou r)
%
\just \igual{ $\ou$ distributivity over $\dimp$ }
%
p \dimp q \dimp p \ou q \dimp r \dimp p \ou r \dimp q\ou r \dimp p \ou q \ou r
%
\just \igual{ $\dimp$ associativity, commutativity}
%
p \dimp q \dimp r \dimp p \ou q  \dimp p \ou r \dimp q\ou r \dimp p \ou q \ou r
%
\end{eqnarray*}

\end{slide} 


\begin{slide}{Example}

\textbf{(cont)}
\begin{eqnarray*}
& & p \dimp q \dimp r \dimp p \ou q  \dimp p \ou r \dimp q\ou r \dimp p \ou q \ou r 
%
\just \igual{ golden rule }
%
(q \e r) \dimp p \dimp p \ou q  \dimp p \ou r \dimp p \ou q \ou r 
%
\just \igual{ $\ou$ distributivity over $\dimp$ }
%
(q \e r) \dimp p \dimp p \ou q  \dimp p \ou (r \dimp q \ou r)
%
\just \igual{ $\ou$ distributivity over $\dimp$ }
%
(q \e r) \dimp p \dimp p \ou (q \dimp r \dimp q \ou r)
%
\just \igual{  golden rule }
%
(q \e r) \dimp p \dimp p \ou  (q \e r)
%
\just \igual{  golden rule }
%
p \e (q \e r)
%
\end{eqnarray*}

\end{slide} 

\begin{slide}{Example}
\begin{center}
\fbox{Theorem: $p \imp q \dimp p \e q \dimp p$}
\end{center}
\begin{eqnarray*}
& & p \imp q \dimp p \e q \dimp p
%
\just \igual{ $\imp$ definition }
%
p \ou q \dimp q \dimp p \e q\dimp p
%
\just \igual{ $\dimp$ associativity, commutativity}
%
(p \dimp q \dimp p \ou q) \dimp p \e q
%
\just \igual{ golden rule }
%
 p \e q \dimp p \e q
%
\end{eqnarray*}

\end{slide} 

\begin{slide}{Example (another proof technique)}
\begin{center}
\fbox{Theorem: $(p \imp q) \imp p \ou r \imp q\ou r$}
\end{center}
\begin{eqnarray*}
& & p \ou r \imp q\ou r
%
\just \igual{ $\imp$ definition }
%
 p \ou r \ou q \ou r \dimp q \ou r
%
\just \igual{ $\ou$ idempotency, $\dimp$ associativity, commutativity}
%
 p \ou  q \ou r \dimp q \ou r
%
\just \igual{ $\ou$ distributivity over $\dimp$ }
%
 (p \ou q \dimp q) \ou r
%
\just \rimp{ weakning: $ p \imp p \ou  q$  }
%
 p \ou q \dimp q
 %
\just \igual{ $\imp$ definition }
%
p \imp q
%
\end{eqnarray*}

\end{slide} 

\begin{slide}{Exercises}
\begin{itemize}
\item $p \ou \false \dimp p$
\item $(p \imp q) \e (q \imp p) \dimp p \dimp q$
\item $(p \imp q) \dimp  \neg p \ou q$
\item $(\neg p \e \neg q)  \ou (q \e p) \dimp p \dimp q$
\end{itemize}
\end{slide} 

\begin{slide}{Resolution}
\small
\begin{center}
\fbox{Theorem: $(p \imp q) \e (q \imp p) \dimp p \dimp q$}
\end{center}
\begin{eqnarray*}
& & (p \imp q) \e (q \imp p)
%
\just \igual{ $\imp$ alternative definition }
%
 (\neg p \ou q) \e (\neg q \ou p)
 %
\just \igual{ $\e,\ou$ distributivity}
%
( (\neg p \ou q) \e \neg q) \ou  (\neg p \ou q) \e p)
%
\just \igual{ $\e,\ou$ distributivity}
%
 (\neg p \e \neg q) \ou (q \e \neg q) \ou (\neg p \e p) \ou (q \e p)
 %
\just \igual{$a \e \neg a \dimp \false$, $a \ou \false \dimp a$}
%
(\neg p \e \neg q)  \ou (q \e p)
%
\just \igual{ Theorem: $(\neg p \e \neg q)  \ou (q \e p) \dimp p \dimp q$}
%
p \dimp q
%
\end{eqnarray*}
\end{slide} 

\begin{slide}{Resolution}
\small
\begin{center}
\fbox{Theorem: $(\neg p \e \neg q)  \ou (q \e p) \dimp p \dimp q$}
\end{center}
\begin{eqnarray*}
& & (\neg p \e \neg q)  \ou (q \e p) 
%
\just \igual{ golden rule }
%
 (\neg p \dimp \neg q \dimp (\neg p \ou \neg q))   \ou (q \e p) 
%
\just \igual{ $\ou$ distributivity}
%
((\neg p \dimp \neg q) \ou (p \e q)) \dimp ((\neg p \ou \neg q) \ou (p \e q))
%
\just \igual{ de Morgan }
%
 ((\neg p \dimp \neg q) \ou (p \e q)) \dimp (\neg (p \e q) \ou (p \e q))
%
\just \igual{excluded middle, $\dimp $ identity}
%
 (\neg p \dimp \neg q) \ou (p \e q)
%
\just \igual{ $\ou$ distributivity}
%
(\neg p \ou (p \e q)) \dimp (\neg q \ou (p \e q)) 
%
\end{eqnarray*}
\end{slide} 

\begin{slide}{Resolution}
\small
(\textbf{cont})
\begin{eqnarray*}
& &(\neg p \ou (p \e q)) \dimp (\neg q \ou (p \e q))  
%
\just \igual{ $\e,\ou$ distributivity}
%
(\neg p \ou p) \e (\neg p \ou q) \dimp (\neg q \ou p) \e (\neg q \ou q)
%
\just \igual{excluded middle, $\true \e a \dimp a$}
%
 (\neg p \ou q) \dimp (\neg q \ou p)
%
\just \igual{theorem: $a \ou b \dimp a \ou \neg b \dimp a$}
%
 (\neg p \ou q) \dimp (q \ou p) \dimp p
%
\just \igual{ $\e,\ou$ distributivity}
%
q \dimp (p \ou \neg p) \dimp p
%
\just \igual{ excluded middle, $\dimp$ identity}
%
q  \dimp p
%
\end{eqnarray*}
\end{slide} 


\begin{slide}{Resolution}
\small
\begin{center}
\fbox{Theorem: $\neg (p \e q)  \dimp \neg q \ou \neg p$}
\end{center}
\begin{eqnarray*}
& & \neg (p \e q) 
%
\just \igual{ golden rule }
%
 \neg (q \dimp p \dimp p \ou q)
%
\just \igual{ $\neg$ distributivity }
%
 \neg q \dimp p \dimp p \ou q
%
\just \igual{ $a \ou \false \dimp a$}
%
\neg q \dimp p \ou \false \dimp p \ou q
%
\just \igual{ $\ou$ distributivity }
%
 \neg q \dimp  (\false \dimp q)  \ou p
%
\just \igual{$\neg a \dimp (\false \dimp a)$}
%
 \neg q  \dimp  \neg q  \ou p
%
\end{eqnarray*}
\end{slide} 


\begin{slide}{Resolution}
\small
(\textbf{cont})
\begin{eqnarray*}
& & \neg q  \dimp  \neg q  \ou p
%
\just \igual{ $a \ou \false \dimp a$}
%
\neg q \ou \false  \dimp  \neg q  \ou p
%
\just \igual{ $\ou$ distributivity}
%
\neg q \ou (\false \dimp p)
%
\just \igual{$\neg a \dimp (\false \dimp a)$}
%
\neg q \ou \neg p
%
\end{eqnarray*}
\end{slide} 




\begin{slide}{}
  ~\\[-15mm]
  \begin{align*}
\text{($\dimp$ associativity)} && ((p \dimp q) \dimp r) &~~\dimp~~ (p \dimp (q \dimp r))\\
\text{($\dimp$ commutativity)} &&  p \dimp q &~~\dimp~~ q \dimp p \\
\text{($\dimp$ identity)} &&  \true &~~\dimp~~ q \dimp q\\
\text{($\false$ definition)} && \false &~~\dimp~~ \neg \true\\
\text{($\neg$ distributivity over $\dimp$)} &&  \neg(p \dimp q) &~~\dimp~~ \neg p \dimp q\\
\text{($\not\equiv$ definition)} &&  (p \not\equiv q) &~~\dimp~~ \neg(p \dimp q)\\
\text{($\e$ negation)} && \neg (p \e q) &~~\dimp~~ (\neg p \ou \neg q)\\
\text{($\ou$ negation)} && \neg (p \ou q) &~~\dimp~~ (\neg p \e \neg q)\\
\text{($\ou$ commutativity)} && p \ou q &~~\dimp~~ q \ou p\\
\text{($\ou$ associativity)} && (p \ou q) \ou r &~~\dimp~~ p\ou (q \ou r)\\
\text{($\ou$ idempotency)} && p \ou p &~~\dimp~~ p\\
\text{($\ou$ distributivity over $\dimp$)} &&  p \ou (q \dimp r) &~~\dimp~~ (p\ou q) \dimp (p \ou r)  \\
\text{(excluded middle)} &&  p \ou \neg p &~~\dimp~~ \true \\
\text{(golden rule)} && p \e q &~~\dimp~~ p \dimp q \dimp p \ou q\\
\text{($\imp$ definition)} && p \imp q &~~\dimp~~ p \ou q \dimp q\\
\text{(consequence)} &&  p \rimp q &~~\dimp~~ q \imp p
  \end{align*}
\end{slide}



%%%%%%%%%%%%%%%%%%%%%%%%%%%%%%%%%%%%%%

\end{document}
